bsearch: WIP absint integration

bedrock2/src/Examples/bsearch.v
@@ -7,7 +7,297 @@ Definition bsearch := @Demos.bsearch _ Demos.BinarySearch.StringNames.Inst.
 From coqutil Require Import Word.Interface Map.Interface. (* coercions word and rep *)
 From bedrock2 Require Import Semantics BasicC64Semantics.
 
+From coqutil Require Import Z.div_mod_to_equations.
 From coqutil.Tactics Require Import syntactic_unify.
+From coqutil.Tactics Require Import rdelta.
+
+  (** Bounds propagation *)
+
+  Lemma Z__range_add a0 a a1 (Ha: a0 <= a < a1) b0 b b1 (Hb : b0 <= b < b1)
+        : a0+b0 <= a+b < a1 + b1 - 1.
+  Proof. Lia.nia. Qed.
+  Lemma Z__range_sub a0 a a1 (Ha: a0 <= a < a1) b0 b b1 (Hb : b0 <= b < b1)
+        : a0-b1+1 <= a-b < a1 - b0.
+  Proof. Lia.nia. Qed.
+  Lemma Z__range_div_pos_const_r n0 n n1 (Hn : n0 <= n < n1) d (Hd : 0 < d)
+    : n0/d <= n/d < n1/d + 1.
+  Proof. Z.div_mod_to_equations. Lia.nia. Qed.
+  Lemma Z__range_mul_nonneg a0 a a1 (Ha: a0 <= a < a1) b0 b b1 (Hb : b0 <= b < b1) (Ha0 : 0 <= a0) (Hb0 : 0 <= b0)
+        : a0*b0 <= a*b < (a1-1)*(b1-1) + 1.
+  Proof. Lia.nia. Qed.
+  Lemma boundscheck {x0 x x1} (H: x0 <= x < x1) {X0 X1} (Hcheck : andb (X0 <=? x0) (x1 <=? X1) = true) : X0 <= x < X1.
+  Proof. eapply andb_prop in Hcheck; case Hcheck; intros H1 H2; eapply Z.leb_le in H1; eapply Z.leb_le in H2. Lia.lia. Qed.
+  Lemma boundscheck_lt {x0 x x1} (H: x0 <= x < x1) {X1} (Hcheck: Z.ltb x1 X1 = true) : x < X1.
+  Proof. eapply Z.ltb_lt in Hcheck. Lia.lia. Qed.
+  Lemma bounded_constant c : c <= c < c+1. Proof. Lia.lia. Qed.
+
+  Ltac named_pose_proof pf :=
+    let H := fresh in
+    let __ := match constr:(Set) with _ => pose proof pf as H end in
+    H.
+  Ltac named_pose pf :=
+    let H := fresh in
+    let __ := match constr:(Set) with _ => pose pf as H end in
+    H.
+  Ltac named_pose_asfresh pf x :=
+    let H := fresh x in
+    let __ := match constr:(Set) with _ => pose pf as H end in
+    H.
+
+  Ltac requireZcst z :=
+    lazymatch Coq.setoid_ring.InitialRing.isZcst z with
+    | true => idtac
+    end.
+  Ltac requireZcstExpr e :=
+    match e with
+    | Z.pred ?x => requireZcstExpr x
+    | Z.succ ?x => requireZcstExpr x
+    | Z.ones ?x => requireZcstExpr x
+    | Z.opp ?x => requireZcstExpr x
+    | Z.lnot ?x => requireZcstExpr x
+    | Z.add ?x ?y => requireZcstExpr x; requireZcstExpr y
+    | Z.sub ?x ?y => requireZcstExpr x; requireZcstExpr y
+    | Z.mul ?x ?y => requireZcstExpr x; requireZcstExpr y
+    | Z.div ?x ?y => requireZcstExpr x; requireZcstExpr y
+    | Z.modulo ?x ?y => requireZcstExpr x; requireZcstExpr y
+    | Z.quot ?x ?y => requireZcstExpr x; requireZcstExpr y
+    | Z.rem ?x ?y => requireZcstExpr x; requireZcstExpr y
+    | Z.pow ?x ?y => requireZcstExpr x; requireZcstExpr y
+    | Z.shiftl ?x ?y => requireZcstExpr x; requireZcstExpr y
+    | Z.shiftr ?x ?y => requireZcstExpr x; requireZcstExpr y
+    | Z.land ?x ?y => requireZcstExpr x; requireZcstExpr y
+    | Z.lor ?x ?y => requireZcstExpr x; requireZcstExpr y
+    | Z.lxor ?x ?y => requireZcstExpr x; requireZcstExpr y
+    | Z.ldiff ?x ?y => requireZcstExpr x; requireZcstExpr y
+    | Z.clearbit ?x ?y => requireZcstExpr x; requireZcstExpr y
+    | Z.setbit ?x ?y => requireZcstExpr x; requireZcstExpr y
+    | Z.min ?x ?y => requireZcstExpr x; requireZcstExpr y
+    | Z.max ?x ?y => requireZcstExpr x; requireZcstExpr y
+    | Z.gcd ?x ?y => requireZcstExpr x; requireZcstExpr y
+    | Z.lcm ?x ?y => requireZcstExpr x; requireZcstExpr y
+    | _ => requireZcst e
+    end.
+
+  Ltac zsimp x :=
+    match constr:(Set) with
+    | _ => let __ := requireZcstExpr x in let y := eval cbv in x in y
+    | _ => x
+    end.
+
+  Local Notation "zbsimp! H" :=
+    (ltac:(
+       lazymatch type of H with
+             ?L <= ?X < ?R =>
+             let L := zsimp L in
+             let R := zsimp R in
+             exact ((H : L <= X < R))
+           end
+    )) (at level 10, only parsing).
+
+  Ltac rbounded e :=
+    let re := rdelta e in
+    match goal with
+    | H :  _ <= e < _ |- _ => H
+    | _ =>
+      match re with
+      | word.unsigned ?a =>
+        named_pose_proof (zbsimp! (Properties.word.unsigned_range a : _ <= e < _))
+      | Z.div ?a ?b => (* TODO: non-constant denominator? *)
+        let __ := match constr:(Set) with _ => requireZcstExpr b end in
+        let Ha := rbounded a in
+        named_pose_proof (zbsimp! (Z__range_div_pos_const_r _ a _ Ha b ltac:(eapply Z.ltb_lt; exact eq_refl) : _ <= e < _))
+      | Z.modulo ?a ?b => (* TODO: non-constant denominator? *)
+        let __ := match constr:(Set) with _ => requireZcstExpr b end in
+        named_pose_proof (zbsimp! (Z.mod_pos_bound a b ltac:(eapply Z.ltb_lt; exact eq_refl) : _ <= e < _))
+      | ?op ?a ?b =>
+        let Ha := rbounded a in
+        let Hb := rbounded b in
+        let a0 := match type of Ha with ?a0 <= _ < ?a1 => a0 end in
+        let a1 := match type of Ha with ?a0 <= _ < ?a1 => a1 end in
+        let b0 := match type of Hb with ?b0 <= _ < ?b1 => b0 end in
+        let b1 := match type of Hb with ?b0 <= _ < ?b1 => b1 end in
+        match op with
+        | Z.add => named_pose_proof (zbsimp! (Z__range_add a0 a a1 Ha b0 b b1 Hb : a0 + b0 <= e < a1 + b1 - 1))
+        | Z.sub => named_pose_proof (zbsimp! (Z__range_sub a0 a a1 Ha b0 b b1 Hb : a0-b1+1 <= e < a1-b0))
+        | Z.mul => named_pose_proof (zbsimp! (Z__range_mul_nonneg a0 a a1 Ha b0 b b1 Hb (Zle_bool_imp_le 0 a0 eq_refl) (Zle_bool_imp_le 0 b0 eq_refl) : _ <= e < _))
+        (* TODO: pow *)
+        (* TODO: and, or, xor, ndn *)
+        end
+      end
+    | _ =>
+      let __ := match constr:(Set) with _ => requireZcstExpr re end in
+      constr:(zbsimp! (bounded_constant e))
+    end.
+
+  (** Abstract interpretation *)
+
+  Module unsigned.
+
+  Definition absint_eq {T} := @eq T.
+  Local Infix "=~>" := absint_eq (at level 70, no associativity).
+    
+  Local Notation "absint_lemma! pf" := (ltac:(
+    cbv [absint_eq] in *;
+    etransitivity; [ eapply pf | ]; cycle -1;
+      [unshelve (repeat match goal with
+        | |-context [Z.shiftr ?x (word.unsigned ?y)] => assert_fails(is_evar x||is_evar y);
+          setoid_rewrite (Z.shiftr_div_pow2 x (word.unsigned y) (proj1 (Properties.word.unsigned_range _)))
+        | |-context [Z.shiftl ?x (word.unsigned ?y)] => assert_fails(is_evar x||is_evar y);
+          setoid_rewrite (Z.shiftl_mul_pow2 x (word.unsigned y) (proj1 (Properties.word.unsigned_range _)))
+        | |-context [?x mod (2^?y)] => assert_fails(is_evar x||is_evar y);
+          rewrite (Z.mod_small x (2^y)) by shelve
+        | |-context [word.unsigned ?x] => assert_fails(is_evar x);
+          erewrite (_:word.unsigned _=_) by shelve
+        end; exact eq_refl)
+      |..];
+      (* WHY do I need [> here? *)
+      [> (repeat match goal with
+                 | H: ?P |- ?G => assert_fails (has_evar P || has_evar G); rewrite H
+                 end;
+          match reverse goal with H : ?e |- ?G => is_evar e; unify e G; exact H end).. ]
+    )) (at level 10, only parsing).
+  
+  Lemma absint_of_Z (x : Z) (Hrange : 0 <= x < 2^width) : word.unsigned (word.of_Z x) = x.
+  Proof. rewrite word.unsigned_of_Z, Z.mod_small; trivial. Qed.
+  Definition absint_add (x y : word.rep) ux Hx uy Hy Hbounds : word.unsigned _ =~> _ :=
+    absint_lemma! (word.unsigned_add x y).
+  Definition absint_sub (x y : word.rep) ux Hx uy Hy Hbounds : word.unsigned _ =~> _ :=
+    absint_lemma! (word.unsigned_sub x y).
+  Definition absint_mul (x y : word.rep) ux Hx uy Hy Hbounds : word.unsigned _ =~> _ :=
+    absint_lemma! (word.unsigned_mul x y).
+  Definition absint_and (x y : word.rep) ux Hx uy Hy : word.unsigned _ =~> _ :=
+    absint_lemma! (Properties.word.unsigned_and_nowrap x y).
+  Definition absint_or (x y : word.rep) ux Hx uy Hy : word.unsigned _ =~> _ :=
+    absint_lemma! (Properties.word.unsigned_or_nowrap x y).
+  Definition absint_xor (x y : word.rep) ux Hx uy Hy : word.unsigned _ =~> _ :=
+    absint_lemma! (Properties.word.unsigned_xor_nowrap x y).
+  Definition absint_ndn (x y : word.rep) ux Hx uy Hy : word.unsigned _ =~> _ :=
+    absint_lemma! (Properties.word.unsigned_ndn_nowrap x y).
+  Definition absint_sru (x y : word.rep) ux Hx uy Hy Hshift  : word.unsigned _ =~> _ :=
+    absint_lemma! (Properties.word.unsigned_sru_nowrap x y).
+  Definition absint_slu (x y : word.rep) ux Hx uy Hy Hrange Hshift : word.unsigned _ =~> _ :=
+    absint_lemma! (word.unsigned_slu x y).
+  Definition absint_divu (x y : word.rep) ux Hx uy Hy Hnz  : word.unsigned _ =~> _ :=
+    absint_lemma! (Properties.word.unsigned_divu_nowrap x y).
+  Definition absint_modu (x y : word.rep) ux Hx uy Hy Hnz  : word.unsigned _ =~> _ :=
+    absint_lemma! (Properties.word.unsigned_modu_nowrap x y).
+
+  Ltac named_pose_asfresh_or_id x n :=
+    let y := match constr:(Set) with _ => named_pose_asfresh x n | _ => x end in
+    y.
+
+  Definition absint_eq_refl {T} v := ((@eq_refl T v) : @absint_eq T v v).
+  Ltac zify_expr e :=
+    let re := rdelta e in
+    lazymatch type of e with
+    | @word.rep ?width ?word_parameters =>
+      match re with
+      | _ => match goal with H: word.unsigned e =~> _ |- _ => H end
+      | word.of_Z ?a =>
+        let Ba := rbounded a in
+        named_pose_proof (absint_of_Z a (boundscheck (X0:=0) (X1:=2^width) Ba (eq_refl true)) : @absint_eq Z (@word.unsigned _ word_parameters e) a)
+      | ?op ?a ?b =>
+        let Ha := zify_expr a in let Ra := lazymatch type of Ha with _ =~> ?x => x end in
+        let Hb := zify_expr b in let Rb := lazymatch type of Hb with _ =~> ?x => x end in
+        match op with
+        | word.and =>
+          named_pose_proof constr:(absint_and a b Ra Ha Rb Hb : @absint_eq Z (@word.unsigned _ word_parameters e) (Z.land Ra Rb))
+        | word.or =>
+          named_pose_proof constr:(absint_or a b Ra Ha Rb Hb : @absint_eq Z (@word.unsigned _ word_parameters e) (Z.lor Ra Rb))
+        | word.xor =>
+          named_pose_proof constr:(absint_xor a b Ra Ha Rb Hb : @absint_eq Z (@word.unsigned _ word_parameters e) (Z.lxor Ra Rb))
+        | word.ndn =>
+          named_pose_proof constr:(absint_ndn a b Ra Ha Rb Hb : @absint_eq Z (@word.unsigned _ word_parameters e) (Z.ldiff Ra Rb))
+
+        | word.add =>
+          let Re := named_pose_asfresh_or_id constr:(Ra+Rb) e in
+          let Be := rbounded Re in
+          let Hbounds := match type of Be with ?x0 <= ?x < ?x1 =>
+                           constr:(@boundscheck x0 x x1 Be 0 (2^width) (@eq_refl bool true)) end in
+          named_pose_proof constr:(absint_add a b Ra Ha Rb Hb Hbounds : @absint_eq Z (@word.unsigned _ word_parameters e) Re)
+        | word.sub =>
+          let Re := named_pose_asfresh_or_id constr:(Ra-Rb) e in
+          let Be := rbounded Re in
+          let Hbounds := match type of Be with ?x0 <= ?x < ?x1 =>
+                           constr:(@boundscheck x0 x x1 Be 0 (2^width) (@eq_refl bool true)) end in
+          named_pose_proof constr:(absint_sub a b Ra Ha Rb Hb Hbounds : @absint_eq Z (@word.unsigned _ word_parameters e) Re)
+        | word.mul =>
+          let Re := named_pose_asfresh_or_id constr:(Ra*Rb) e in
+          let Be := rbounded Re in
+          let Hbounds := match type of Be with ?x0 <= ?x < ?x1 =>
+                           constr:(@boundscheck x0 x x1 Be 0 (2^width) (@eq_refl bool true)) end in
+          named_pose_proof constr:(absint_mul a b Ra Ha Rb Hb Hbounds : @absint_eq Z (@word.unsigned _ word_parameters e) Re)
+
+        | word.sru =>
+          let Re := named_pose_asfresh_or_id constr:((Ra / 2^Rb)) e in
+          let Bb := rbounded Rb in
+          let pf := constr:(absint_sru a b Ra Ha Rb Hb (@boundscheck_lt _ Rb _ Bb width eq_refl): @absint_eq Z (@word.unsigned _ word_parameters e) Re) in
+          named_pose_proof pf
+        | word.slu =>
+          let Re := named_pose_asfresh_or_id constr:((Ra * 2^Rb)) e in
+          let Bb := rbounded Rb in
+          let Be := rbounded Re in
+          named_pose_proof (absint_slu a b Ra Ha Rb Hb (boundscheck (X0:=0) (X1:=2^width) Be (eq_refl true)) (@boundscheck_lt _ Rb _ Bb width eq_refl): @absint_eq Z (@word.unsigned _ word_parameters e) Re)
+        | _ => (* unknown binop or bad bounds, don't backtrack to keep Ha and Hb *)
+          constr:(@absint_eq_refl Z (@word.unsigned _ word_parameters e))
+         (* TODO: divu, modu (how do we prove denominator nonzero?) *)
+        end
+      | _ =>
+        constr:(@absint_eq_refl Z (@word.unsigned _ word_parameters e))
+      end
+    | Z =>
+      match e with
+      | _ => match goal with H: e =~> _ |- _ => H end
+      | word.unsigned ?a => zify_expr a
+      | _ => constr:(@absint_eq_refl Z e)
+      end
+    end.
+  End unsigned.
+  
+  Import unsigned.
+
+
+
+
+
+  Strategy -1000 [word parameters].
+  Fixpoint goal (x : word) (n : nat) : Prop
+    := match n with
+       | O => True
+       | S n' => let x := word.add x x in goal x n'
+       end.
+  Goal forall x X, 1 <= X < 2^60 -> unsigned.absint_eq (word.unsigned x) X -> goal x 7.
+  Proof.
+    cbv beta iota delta [goal].
+    intros.
+
+    let e := match goal with x := _ |- _ => x end in
+    let e := constr:(word.ndn (word.xor (word.or (word.and (word.sub (word.mul (word.slu (word.sru e (word.of_Z 16)) (word.of_Z 3)) x) x) x) x) x) x) in
+    let H := unsigned.zify_expr e in
+    idtac H.
+    exact I.
+  Qed.
+
+
+
+  Goal forall x y, 0 <= x < 5 -> 10 <= y < 20 -> True.
+  Proof.
+    intros.
+  
+    set (a := x+y).
+    set (b := y+x).
+    set (c := a*b+7).
+  
+    let e := constr:(a + y mod 2 * (b*(x*y/4)) + c) in
+    let H := rbounded e in
+    cbn in *.
+  
+    let e := constr:(a*c + b) in
+    let H := rbounded e in
+    idtac H;
+    cbn in *.
+    exact I.
+  Qed.
 
 (* custom rewrite tactic to work around COQBUG(4885) *)
 Ltac set_evars := repeat match goal with |- context[?e] => is_evar e; set e end.
@@ -49,6 +339,8 @@ Proof.
   apply Properties.word.wrap_unsigned.
 Qed.
 
+  From coqutil Require Import Z.div_mod_to_equations.
+
 Monomorphic Definition word__monomorphic_ring_theory := Properties.word.ring_theory.
 Add Ring word_ring : word__monomorphic_ring_theory.
 
@@ -67,7 +359,6 @@ From coqutil.Tactics Require Import eabstract letexists rdelta.
 From coqutil.Macros Require Import symmetry.
 Import PrimitivePair.
 
-From coqutil Require Import Z.div_mod_to_equations.
 
 Axiom __mem_ok : map.ok mem. Local Existing Instance __mem_ok.
 
@@ -103,14 +394,75 @@ Proof.
   { repeat straightline.
     2: solve [auto]. (* exiting loop *)
     (* loop body *)
+    rename H3 into length_rep. subst br. subst v0.
+    cbn [interp_binop] in *.
     seprewrite @array_address_inbounds.
-    1: admit. 1: admit. 1: exact eq_refl.
-    (* if expression *)  letexists; split. 1: repeat straightline. (* determines element *)
+    all: (* if expression *) [> ..|exact eq_refl|letexists; split; [repeat straightline|]]. (* determines element *)
+    { rewrite word__add_sub.
+      repeat match goal with |- context[word.unsigned ?e] => let H := unsigned.zify_expr e in rewrite H end.
+      rewrite length_rep in *. (* WHY is this necessary for lia? *)
+      Z.div_mod_to_equations. Lia.lia. }
+    { rewrite word__add_sub.
+      repeat match goal with |- context[word.unsigned ?e] => let H := unsigned.zify_expr e in rewrite H end.
+      Z.div_mod_to_equations. Lia.lia. }
     (* split if cases *) split; repeat straightline. (* code is processed, loop-go-again goals left behind *)
     { repeat letexists. split. 1: repeat straightline.
       repeat letexists; repeat split; repeat straightline.
-      { cbn [interp_binop] in *. subst v2; subst x7. SeparationLogic.ecancel_assumption. }
-      { cbn [interp_binop] in *. subst v2; subst x7. subst v0.
+      { cbn [interp_binop] in *. subst v1; subst x7. SeparationLogic.ecancel_assumption. }
+      { cbn [interp_binop] in *.
+        lazymatch goal with |- word.unsigned ?e = _ => let H := unsigned.zify_expr e in idtac H end.
+        subst v1; subst x7. subst v0.
         repeat ureplace (_:word) by (set_evars; progress ring_simplify; subst_evars; exact eq_refl).
+        rewrite H13.
+        unshelve erewrite (_ : forall xs, Datatypes.length xs <> 0%nat -> Datatypes.length (List.tl xs) = pred (Datatypes.length xs)). admit.
+        unshelve erewrite (_ : forall xs delta, (Datatypes.length xs > delta)%nat -> Datatypes.length (List.skipn delta xs) = (Datatypes.length xs - delta)%nat). admit.
+        unshelve erewrite (_ : forall n, n <> O -> Z.of_nat (Init.Nat.pred n) = Z.of_nat n - 1). { clear. intros. Lia.lia. }
+        rewrite Nat2Z.inj_sub, Z2Nat.id.
+        rewrite word.unsigned_sub, Z.mod_small.
+        rewrite word.unsigned_sub, Z.mod_small.
+        rewrite H12.
+        setoid_rewrite H13.
+        setoid_rewrite length_rep.
+        change (2^4) with 16.
+        rewrite Z.div_mul by discriminate.
+        Lia.lia.
+        admit.
+        admit.
+        admit.
+        admit.
+        admit.
+        admit.
+        admit. }
+      { subst v'; subst v. subst x7. admit. }
 
+      cbn [interp_binop] in *.
+      subst x8. SeparationLogic.seprewrite_in (symmetry! @array_address_inbounds) H7.
+
+      { rewrite word__add_sub.
+        destruct x; cbn [Datatypes.length] in *.
+        { rewrite Z.mul_0_r in length_rep. Lia.lia. }
+        repeat match goal with |- context[word.unsigned ?e] => let H := unsigned.zify_expr e in rewrite H end.
+        rewrite length_rep.  clear. Z.div_mod_to_equations. Lia.lia. }
+      { rewrite word__add_sub.
+        repeat match goal with |- context[word.unsigned ?e] => let H := unsigned.zify_expr e in rewrite H end.
+        rewrite length_rep.  clear. Z.div_mod_to_equations. Lia.lia. }
+      { exact eq_refl. }
+      { SeparationLogic.ecancel_assumption. } }
+    (* second branch of the if, very similar goals... *)
+    { repeat letexists. split. 1: solve [repeat straightline].
+      repeat letexists; repeat split; repeat straightline.
+      { cbn [interp_binop] in *. subst v1; subst x7; subst x8. SeparationLogic.ecancel_assumption. }
+      { admit. }
+      { subst v. subst v'. subst x7. admit. }
+      subst x8. SeparationLogic.seprewrite_in (symmetry! @array_address_inbounds) H7.
+      1: admit. 1: admit. 1: exact eq_refl.
+      SeparationLogic.ecancel_assumption. } }
+
+  repeat straightline.
+  repeat apply conj; auto; []. (* postcondition *)
+  letexists. split.
+  { exact eq_refl. }
+  { auto. }
+
+  all:fail "remaining subgoals".
 Admitted.
